---
interact_link: notebooks/Chapter_08/03_Expectations_of_Functions.ipynb
title: '8.3 Expectations of Functions'
permalink: 'chapters/Chapter_08/03_Expectations_of_Functions'
previouschapter:
  url: chapters/Chapter_08/02_Additivity
  title: '8.2 Additivity'
nextchapter:
  url: chapters/Chapter_08/04_Review_Problems_Set_2
  title: '8.4 Review Problems: Set 2'
redirect_from:
  - 'chapters/chapter-08/03-expectations-of-functions'
---

## Expectations of Functions

Once we start using random variables as estimators, we will want to see how far the estimate is from a desired value. For example, we might want to see how far a random variable $X$ is from the number 10. That's a function of $X$. Let's call it $Y$. Then

$$
Y = |X - 10|
$$

which is not a linear function. To find $E(Y)$, we need a bit more technique. Throughout, we will assume that all the expectations that we are discussing are well defined.

This section is about finding the expectation of a function of a random variable whose distribution you know.

In what follows, let $X$ be a random variable whose distribution (and hence also expectation) are known.

### Linear Function Rule
Let $Y = aX + b$ for some constants $a$ and $b$. In an earlier section we showed that

$$
E(Y) = aE(X) + b
$$

This includes the case where $a=0$ and thus $Y$ is just the constant $b$ and thus has expectation $b$.

### Non-linear Function Rule
Now let $Y = g(X)$ where $g$ is any numerical function. Remember that $X$ is a function on $\Omega$. So the function that defines the random variable $Y$ is a *composition*:

$$
Y(\omega) = (g \circ X) (\omega) ~~~~~~~~~ \text{for } \omega \in \Omega
$$

This allows us to write $E(Y)$ in three equivalent ways:

#### On the range of $Y$

$$
E(Y) =  \sum_{\text{all }y} yP(Y=y)
$$

#### On the domain $\Omega$

$$
E(Y) = E(g(X)) = \sum_{\omega \in \Omega} (g \circ X) (\omega) P(\omega)
$$

#### On the range of $X$

$$
E(Y) = E(g(X)) = \sum_{\text{all }x} g(x)P(X=x)
$$

As before, it is a straightforward matter of grouping to show that all the forms are equivalent.

The first form looks the simplest, but there's a catch: you need to first find $P(Y=y)$. The second form involves an unnecessarily high level of detail.

The third form is the one to use. It uses the known distribution of $X$. It says that to find $E(Y)$ where $Y = g(X)$ for some function $g$:
- Take a generic value $x$ of $X$.
- Apply $g$ to $x$; this $g(x)$ is a generic value of $Y$.
- Weight $g(x)$ by $P(X=x)$, which is known.
- Do this for all $x$ and add. The sum is $E(Y)$.

The crucial thing to note about this method is that **we didn't have to first find the distribution of $Y$**. That saves us a lot of work. Let's see how our method works in some examples.

### Example 1: $Y = \vert X-3 \vert$
Let $X$ have a distribution we worked with earlier:



{:.input_area}
```python
x = np.arange(1, 6)
probs = make_array(0.15, 0.25, 0.3, 0.2, 0.1)
dist = Table().values(x).probability(probs)
dist = dist.relabel('Value', 'x').relabel('Probability', 'P(X=x)')
dist
```





<div markdown="0">
<table border="1" class="dataframe">
    <thead>
        <tr>
            <th>x</th> <th>P(X=x)</th>
        </tr>
    </thead>
    <tbody>
        <tr>
            <td>1   </td> <td>0.15  </td>
        </tr>
        <tr>
            <td>2   </td> <td>0.25  </td>
        </tr>
        <tr>
            <td>3   </td> <td>0.3   </td>
        </tr>
        <tr>
            <td>4   </td> <td>0.2   </td>
        </tr>
        <tr>
            <td>5   </td> <td>0.1   </td>
        </tr>
    </tbody>
</table>
</div>



Let $g$ be the function defined by $g(x) = \vert x-3 \vert$, and let $Y = g(X)$. In other words, $Y = \vert X - 3 \vert$. 

To calculate $E(Y)$, we first have to create a column that transforms the values of $X$ into values of $Y$:



{:.input_area}
```python
dist_with_Y = dist.with_column('g(x)', np.abs(dist.column('x')-3)).move_to_end('P(X=x)')

dist_with_Y
```





<div markdown="0">
<table border="1" class="dataframe">
    <thead>
        <tr>
            <th>x</th> <th>g(x)</th> <th>P(X=x)</th>
        </tr>
    </thead>
    <tbody>
        <tr>
            <td>1   </td> <td>2   </td> <td>0.15  </td>
        </tr>
        <tr>
            <td>2   </td> <td>1   </td> <td>0.25  </td>
        </tr>
        <tr>
            <td>3   </td> <td>0   </td> <td>0.3   </td>
        </tr>
        <tr>
            <td>4   </td> <td>1   </td> <td>0.2   </td>
        </tr>
        <tr>
            <td>5   </td> <td>2   </td> <td>0.1   </td>
        </tr>
    </tbody>
</table>
</div>



To get $E(Y)$, find the appropriate weighed average: multiply the `g(x)` and `P(X=x)` columns, and add. The calculation shows that $E(Y) = 0.95$.



{:.input_area}
```python
ev_Y = sum(dist_with_Y.column('g(x)') * dist_with_Y.column('P(X=x)'))
ev_Y
```





{:.output_data_text}
```
0.94999999999999996
```



### Example 2: $Y = \min(X, 3)$
Let $X$ be as above, but now let $Y = \min(X, 3)$. We want $E(Y)$. What we know is the distribution of $X$:



{:.input_area}
```python
dist
```





<div markdown="0">
<table border="1" class="dataframe">
    <thead>
        <tr>
            <th>x</th> <th>P(X=x)</th>
        </tr>
    </thead>
    <tbody>
        <tr>
            <td>1   </td> <td>0.15  </td>
        </tr>
        <tr>
            <td>2   </td> <td>0.25  </td>
        </tr>
        <tr>
            <td>3   </td> <td>0.3   </td>
        </tr>
        <tr>
            <td>4   </td> <td>0.2   </td>
        </tr>
        <tr>
            <td>5   </td> <td>0.1   </td>
        </tr>
    </tbody>
</table>
</div>



To find $E(Y)$ we can just go row by row and replace the value of $x$ by the value of $\min(x, 3)$, and then find the weighted average:



{:.input_area}
```python
ev_Y = 1*0.15 + 2*0.25 + 3*0.3 + 3*0.2 + 3*0.1
ev_Y
```





{:.output_data_text}
```
2.45
```



### Example 3: $E(X^2)$ for a Poisson Variable $X$
Let $X$ have the Poisson $(\mu)$ distribution. You will see in the next chapter that it will be useful to know the value of $E(X^2)$. By our non-linear function rule,

$$
E(X^2) = \sum_{k=0}^\infty k^2 e^{-\mu} \frac{\mu^k}{k!}
$$

This sum turns out to be hard to simplify. The term for $k=0$ is 0. In each term for $k \ge 1$, one of the $k$'s in the numerator cancels a $k$ in the denominator but the other factor of $k$ in the numerator remains. It would be so nice if that factor $k$ were $k-1$ instead, so it could cancel $k-1$ in the denominator.

This motivates the following calculation. No matter what $X$ is, if we know $E(X)$ and can find $E(X(X-1))$, then we can use additivity to find $E(X^2)$ as follows:

$$
E(X(X-1)) = E(X^2 - X) = E(X^2) - E(X) 
$$

so

$$
E(X^2) = E(X(X-1)) + E(X)
$$

Let's see if we can find $E(X(X-1))$ by applying the non-linear function rule.

$$
\begin{align*}
E(X(X-1)) &= \sum_{k=0}^\infty k(k-1) e^{-\mu} \frac{\mu^k}{k!} \\ \\
&= e^{-\mu} \mu^2 \sum_{k=2}^\infty \frac{\mu^{k-2}}{(k-2)!} \\ \\
&= e^{-\mu}\mu^2 e^\mu \\ \\
&= \mu^2
\end{align*}
$$

We know that $E(X) = \mu$, so

$$
E(X^2) = \mu^2 + \mu
$$

Notice that $E(X^2) > (E(X))^2$. This is an instance of a general fact. Later in the course we will see why it matters.

For now, as an exercise, see if you can find $E(X(X-1)(X-2))$ and hence $E(X^3)$.
